src/goose_lang/interpreter/generated_test.v
@@ -103,6 +103,8 @@ Example testShiftMod_ok : testShiftMod #() ~~> #true := t.
 (* prims.go *)
 Example testLinearize_ok : testLinearize #() ~~> #true := t.
 
+(* semantics.actual.v *)
+
 (* shortcircuiting.go *)
 Example testShortcircuitAndTF_ok : testShortcircuitAndTF #() ~~> #true := t.
 Example testShortcircuitAndFT_ok : testShortcircuitAndFT #() ~~> #true := t.
